\documentclass[10pt,a4paper, margin=1in]{article}
\usepackage{fullpage}
\usepackage{amsfonts, amsmath, pifont}
\usepackage{amsthm}
\usepackage{graphicx}
\usepackage{float}
\usepackage{geometry}
\usepackage{tkz-euclide}
\usepackage{tikz}
\usepackage{pgfplots}
\usepackage{amssymb}
\pgfplotsset{compat=1.13}
 \geometry{
 a4paper,
 total={210mm,297mm},
 left=10mm,
 right=10mm,
 top=10mm,
 bottom=10mm,
 }
 % Write both of your names here. Fill exxxxxxx with your ceng mail address.
 \author{
  Burhan, Beste\\
  \texttt{e2171395@ceng.metu.edu.tr}
}
\title{CENG 384 - Signals and Systems for Computer Engineers \\
Spring 2018-2019 \\
Written Assignment 3}
\begin{document}
\maketitle



\noindent\rule{19cm}{1.2pt}

\begin{enumerate}

\item 
    \begin{enumerate}
    % Write your solutions in the following items.
    \item %write the solution of q1a
    \ \\
    N=4\\
    $x[n] = \sum_{k=0}^{3} a_k e^{jk(2\pi/4)n}$\\
    $a_k = \dfrac{1}{4} \sum_{n=0}^{3} x[n] e^{-jk(2\pi/4)n}$\\
    \null \ \ \ \ = $\dfrac{1}{4}(x[0](e^{-jk(\pi/2).0}) + x[1](e^{-jk(\pi/2)}) + x[2](e^{-jk\pi}) + x[3](e^{-jk(3\pi/2)}) )$\\
   \null \ \ \ \ = $\dfrac{1}{4}(0+ e^{-jk\pi/2} + 2 e^{-jk\pi} + e^{-jk3\pi/2})$\\
   \null \ \ \ \ = $\dfrac{1}{4}(e^{-jk\pi/2} + 2 e^{-jk\pi} + e^{-jk3\pi/2})$ \ \ \ \ $0\le k \le 3$ for every 4 period\\
   $a_0=1$\\
   $a_1=-1/2$\\
   $a_2=0$\\
   $a_3=-1/2$\\
   \begin{figure}[h!]
   	\centering
   	\begin{tikzpicture}[scale=1.1] 
   	\begin{axis}[
   	axis lines=middle,
   	xlabel={$k$},
   	ylabel={$\boldsymbol{a_k}$},
   	xtick={ -5,-4,-3,-2,-1,0,1,2,3,4,5},
   	ytick={-2,-1,0,...,1,2},
   	ymin=-2, ymax=2,
   	xmin=-5, xmax=5,
   	every axis x label/.style={at={(ticklabel* cs:1.05)}, anchor=west,},
   	every axis y label/.style={at={(ticklabel* cs:1.05)}, anchor=south,},
   		 ]
   	
   	\addplot [ycomb, black, thick, mark=*] table [x={k}, y={ak}] {q1a.dat};
   	\end{axis}
   	 
   	\end{tikzpicture}
   	\caption{$a_k$}
   	\label{fig:q1}
   \end{figure}\\
	\begin{figure}[h!]
	\centering
	\begin{tikzpicture}[scale=1.1] 
	\begin{axis}[
	axis lines=middle,
	xlabel={$k$},
	ylabel={$\boldsymbol{\sphericalangle a_k}$},
	xtick={ -5,-4,-3,-2,-1,0,1,2,3,4,5},
	ytick={-2,-1,0,...,1,2},
	ymin=-2, ymax=2,
	xmin=-5, xmax=5,
	every axis x label/.style={at={(ticklabel* cs:1.05)}, anchor=west,},
	every axis y label/.style={at={(ticklabel* cs:1.05)}, anchor=south,},
	]
	
	\addplot [ycomb, black, thick, mark=*] table [x={k}, y={ak}] {q1aa.dat};
	\end{axis}
	
	\end{tikzpicture}
	\caption{Phase of $a_k$}
	\label{fig:q1}
	\end{figure}\\
\ \\
\ \\
\ \\
\ \\
\ \\
\ \\
\ \\
\ \\
\ \\
    \item %write the solution of q1b
    \ \\
   \begin{enumerate}
   	\item
   	\ \\
   	$y[n]=x[n]-\sum_{k=-\infty}^{\infty}\delta[n-4k+1]$\\
   	\item
   	\ \\
   	 $y[n] = \sum_{k=0}^{3} a_k e^{jk(2\pi/4)n}$\\
   	  $a_k = \dfrac{1}{4} \sum_{n=0}^{3} y[n] e^{-jk(2\pi/4)n}$\\
   	  \null \ \ \ \ = $\dfrac{1}{4}(y[0](e^{-jk(\pi/2).0}) + y[1](e^{-jk(\pi/2)}) + y[2](e^{-jk\pi}) + y[3](e^{-jk(3\pi/2)}) )$\\
   	  \null \ \ \ \ = $\dfrac{1}{4}(0+ e^{-jk\pi/2} + 2 e^{-jk\pi} +0)$\\
   	  \null \ \ \ \ = $\dfrac{1}{4}(e^{-jk\pi/2} + 2 e^{-jk\pi})$\\
   	  $a_0=3/4$\\
   	  $a_1=\dfrac{-j-2}{4}$\\
   	  $a_2=1/4$\\
   	  $a_3=\dfrac{j-2}{4}$\\
   	     \begin{figure}[h!]
   	  	\centering
   	  	\begin{tikzpicture}[scale=1.1] 
   	  	\begin{axis}[
   	  	axis lines=middle,
   	  	xlabel={$k$},
   	  	ylabel={$\boldsymbol{|a_k|}$},
   	  	xtick={ -5,-4,-3,-2,-1,0,1,2,3,4,5},
   	  	ytick={-2,-1,0,...,1,2},
   	  	ymin=-2, ymax=2,
   	  	xmin=-5, xmax=5,
   	  	every axis x label/.style={at={(ticklabel* cs:1.05)}, anchor=west,},
   	  	every axis y label/.style={at={(ticklabel* cs:1.05)}, anchor=south,},
   	  	]
   	  	
   	  	\addplot [ycomb, black, thick, mark=*] table [x={k}, y={ak}] {q1b.dat};
   	  	\end{axis}
   	  	
   	  	\end{tikzpicture}
   	  	\caption{Magnitude of $a_k$}
   	  	\label{fig:q1}
   	  \end{figure}\\
          \begin{figure}[h!]
     	\centering
     	\begin{tikzpicture}[scale=1.1] 
     	\begin{axis}[
     	axis lines=middle,
     	xlabel={$k$},
     	ylabel={$\boldsymbol{\sphericalangle a_k}$},
     	xtick={ -5,-4,-3,-2,-1,0,1,2,3,4,5},
     	ytick={-2,-1,0,...,1,2},
     	ymin=-2, ymax=2,
     	xmin=-5, xmax=5,
     	every axis x label/.style={at={(ticklabel* cs:1.05)}, anchor=west,},
     	every axis y label/.style={at={(ticklabel* cs:1.05)}, anchor=south,},
     	]
     	
     	\addplot [ycomb, black, thick, mark=*] table [x={k}, y={ak}] {q1bb.dat};
     	\end{axis}
     	
     	\end{tikzpicture}
     	\caption{Phase of $a_k$}
     	\label{fig:q1}
     \end{figure}\\
   	  \ \\
   	  \ \\
   	  
   \end{enumerate}

\end{enumerate}


\item %write the solution of q2
\ \\
	$\sum_{k=-3}^{4} = 8$ \ \ \ \ ..from part b \\
	Since period is 4,\\
	\ \ $x[-3]=x[1],x[-2]=x[2],x[-1]=x[3],x[0]=x[4]$\\
	\ \\
	Therefore;
	\null \ \ \ \ \qquad \ \qquad (1) \ \ \ $x[1]+x[2]+x[3]+x[4]=4$\\
	\ \\
	$\sum_{0}^{3} x[k](e^{-jk\pi/2} + e^{-jk3\pi/2}) = 4$ \ \ \ \ ..from part e\\ 
	\null \qquad \ \qquad \ \qquad \ \qquad \ \qquad\ \ \ \ =$x[0]2+x[1](e^{-j\pi/2} + e^{-j3\pi/2}) + x[2](e^{-j\pi} + e^{-j3\pi}) + x[3](e^{-j3\pi/2} + e^{-j9\pi/2})$\\
	\null \qquad \ \qquad \ \qquad \ \qquad \ \qquad\ \ \ \ =$2x[0]-2x[2]$\\
	\null \qquad \ \qquad \ \qquad \ \qquad \ \qquad\ \ \ \ =$4$\\
	$x[0]-x[2]=2$\\
	since period is 4\\
	\ \\
	Therefore; 	\null \ \ \ \ \qquad \ \qquad (2) \ \ \ $x[4]-x[2]=2$\\
	\ \\
	from part c\\
	$a_{-3}=a_{-15}=a_1$ and $a_{11}=a_3$ because of periodicty of $a_k$ \\
	\null \qquad \ \qquad \ \qquad \qquad \qquad (3) $|a_1-a_3|=1$\\
	\ \\
	\ \\
	$a_1 = \dfrac{1}{4} \sum_{n=1}^{4} x[n]e^{-jn\pi/2} $\\
	\null \ \ \ \ = $\dfrac{1}{4} ( x[1](-j) + x[2](-1) + x[3](j) + x[4](1))$\\
	\ \\
	\ \\
	$a_3 = \dfrac{1}{4} \sum_{n=1}^{4} x[n]e^{-jn3\pi/2} $\\
	\null \ \ \ \ = $\dfrac{1}{4} ( x[1](j) + x[2](-1) + x[3](-j) + x[4](1))$\\
	\ \\
	Since (3) $|a_1-a_3|=1$\\
	\null \quad $a_1-a_3 = \dfrac{2j}{4}(x[3]-x[1])$\\
	\null \qquad \ \qquad \ \qquad \qquad \qquad (4a) $x[3]-x[1]=2$ \quad or \quad (4b) $x[3]-x[1]=-2 $ can be.\\
	Therefore;
	\null \qquad \ \qquad \ \ \ \ \ (5a) $a_1 = \dfrac{j}{2}+\dfrac{1}{2}$  \quad or \quad  (5b) $a_1 = \dfrac{-j}{2}+\dfrac{1}{2}$\\
	\null \qquad \ \qquad \ \qquad \qquad \qquad (6a) $a_3 = \dfrac{-j}{2}+\dfrac{1}{2}$  \quad or \quad (6b) $a_1 = \dfrac{j}{2}+\dfrac{1}{2}$\\
	\ \\
	$a_4 = \dfrac{1}{4} \sum_{n=1}^{4} x[n]e^{-jn2\pi} $\\
	\null \ \ \ \ = $\dfrac{1}{4} ( x[1](1) + x[2](1) + x[3](1) + x[4](1))$\ \ \ \ \ from (1) \ \ \ $x[1]+x[2]+x[3]+x[4]=4$\\
		\null \qquad \ \qquad \ \qquad \qquad \qquad (7) $a_4 = 1$\\
	\ \\
	Since one of the coefficients is zero\\
	 \null \qquad \ \qquad \ \qquad \qquad \qquad  (8) $a_2=0$\\
	 \ \\
	 $a_2 = \dfrac{1}{4} \sum_{n=1}^{4} x[n]e^{-jn\pi} $\\
	 \null \ \ \ \ = $\dfrac{1}{4} ( x[1](-1) + x[2](1) + x[3](-1) + x[4](1))$\\
	 $( x[1](-1) + x[2](1) + x[3](-1) + x[4](1))=0$ and from (1) $x[1]+x[2]+x[3]+x[4]=4$\\
	 \ \\
	 \null \qquad \ \qquad \ \qquad \qquad \qquad (9) $x[3]+x[1]=1$\\
	  and from (4a) $x[3]-x[1]=2$\\
	  \ \\
		\null \qquad \ \qquad ** $x[3]=2$\\
		\null \qquad \ \qquad  ** $x[1]=0$\\
	 \ \\
		\null \qquad \ \qquad  $x[2] = \sum_{k=1}^{4}a_ke^{jk\pi}$\\
	 	\null \qquad \ \qquad \null \ \ \ \quad = $a_1(-1)+a_2(1)+a_3(-1)+a_4(1)$\\
		\null \qquad \ \qquad  **$x[2]$ = 0\\
	 \ \\
		\null \qquad \ \qquad  from (2) $x[4]- x[2]=2$\\
		\null \qquad \ \qquad  ** $x[4]=2$\\
		\begin{figure}[h!]
			\centering
			\begin{tikzpicture}[scale=1.1] 
			\begin{axis}[
			axis lines=middle,
			xlabel={$n$},
			ylabel={$\boldsymbol{x_n}$},
			xtick={ -5,-4,-3,-2,-1,0,1,2,3,4,5},
			ytick={-2,-1,0,...,1,2},
			ymin=-2, ymax=2,
			xmin=-5, xmax=5,
			every axis x label/.style={at={(ticklabel* cs:1.05)}, anchor=west,},
			every axis y label/.style={at={(ticklabel* cs:1.05)}, anchor=south,},
			]
			
			\addplot [ycomb, black, thick, mark=*] table [x={k}, y={ak}] {q2a.dat};
			\end{axis}
			
			\end{tikzpicture}
			\caption{$x_n$}
			\label{fig:q1}
		\end{figure}\\
		\ \\
	 and from (4b) $x[3]-x[1]=-2$\\
	 \ \\
	\null \qquad \ \qquad ** $x[3]=0$\\
	\null \qquad \ \qquad  ** $x[1]=2$\\
	\ \\
	\null \qquad \ \qquad  $x[2] = \sum_{k=1}^{4}a_ke^{jk\pi}$\\
	\null \qquad \ \qquad \null \ \ \ \quad = $a_1(-1)+a_2(1)+a_3(-1)+a_4(1)$\\
	\null \qquad \ \qquad  **$x[2]$ = 0\\
	\ \\
	\null \qquad \ \qquad  from (2) $x[4]- x[2]=2$\\
	\null \qquad \ \qquad  ** $x[4]=2$\\
	\ \\
		\begin{figure}[h!]
		\centering
		\begin{tikzpicture}[scale=1.1] 
		\begin{axis}[
		axis lines=middle,
		xlabel={$x$},
		ylabel={$\boldsymbol{x_n}$},
		xtick={ -5,-4,-3,-2,-1,0,1,2,3,4,5},
		ytick={-2,-1,0,...,1,2},
		ymin=-2, ymax=2,
		xmin=-5, xmax=5,
		every axis x label/.style={at={(ticklabel* cs:1.05)}, anchor=west,},
		every axis y label/.style={at={(ticklabel* cs:1.05)}, anchor=south,},
		]
		
		\addplot [ycomb, black, thick, mark=*] table [x={k}, y={ak}] {q2aa.dat};
		\end{axis}
		
		\end{tikzpicture}
		\caption{$x_n$}
		\label{fig:q1}
	\end{figure}\\
\ \\
\ \\
\ \\
\ \\
\ \\
\ \\
\ \\
\ \\
\ \\
\item  
\ \\
$x(t) = h(t)*x(t)+h(t)*r(t)$ \quad \qquad $\dfrac{-K2\pi}{2} \le w \le \dfrac{K2\pi}{2}$ \\
$X(jw) = H(jw)X(jw) + H(jw)R(jw)$   \quad \qquad $\dfrac{-K2\pi}{2} \le w \le \dfrac{K2\pi}{2}$\\
$R(jw)=0$  for $ \dfrac{-K2\pi}{2} \le w \le \dfrac{K2\pi}{2} $\\
$X(jw) = H(jw)X(jw)$  \quad \qquad $\dfrac{-K2\pi}{2} \le w \le \dfrac{K2\pi}{2}$ \\
$H(jw)=1$  \quad \qquad $\dfrac{-K2\pi}{2} \le w \le \dfrac{K2\pi}{2}$ \\
$h(t) = \delta(t) $  \quad \qquad $\dfrac{-K2\pi}{2} \le w \le \dfrac{K2\pi}{2}$ \\


\item 
\ \\
    \begin{enumerate}
    \item %write the solution of q4a
    \ \\
    $y(t) = \int_{}^{} (4x(t)-5y(t)+(\int (x(t)-6y(t))dt))dt$\\
    $\dfrac{d y(t)}{dt}= 4x(t) - 5y(t) + \int (x(t)-6y(t))dt$\\
    $\dfrac{d^2 y(t)}{dt^2} = \dfrac{4d x(t)}{dt} - \dfrac{5d y(t)}{dt} + x(t) -6y(t)$\\
    $\ddot{y}(t) + 5\dot{y}(t)-6y(t) = x+4\dot{x}(t)$\\
    \ \\
  $Y(jw)=H(jw)X(jw)$\\
  $H(jw)=\dfrac{1+4(jw)}{-6+5(jw)+(jw)^2}$\\
  $H(jw)=\dfrac{1+4(jw)}{(jw-3)(jw-2)}$\\
   \item %write the solution of q4b
  \ \\
  $x(t)=\delta(t)$\\
  $X(jw)=1$\\
  $H(jw)=\dfrac{1+4(jw)}{(jw-3)(jw-2)}= \dfrac{-13}{3-jw}+\dfrac{9}{2-jw}$\\
  $h(t)=(-13e^{3t}+9e^{2t})u(-t)$
  \item %write the solution of q4a
  \ \\
  $X(jw)=\dfrac{1}{4}\dfrac{1}{jw+1/4}=\dfrac{1}{(4jw+1)}$\\
   $Y(jw)=H(jw)X(jw)$\\
   $Y(jw)=\dfrac{1+4(jw)}{-6+5(jw)+(jw)^2}.\dfrac{1}{(4jw+1)}$\\
   $Y(jw)=\dfrac{1}{(jw-3)(jw-2)}=\dfrac{-1}{3-jw}+\dfrac{1}{2-jw}$\\
 $y(t)= (e^{2t}-e^{3t})u(-t)$
    \end{enumerate}



\end{enumerate}
\end{document}

