\documentclass[10pt,a4paper, margin=1in]{article}
\usepackage{fullpage}
\usepackage{amsfonts, amsmath, pifont}
\usepackage{amsthm}
\usepackage{graphicx}
\usepackage{float}
\usepackage{geometry}
\usepackage{tkz-euclide}
\usepackage{tikz}
\usepackage{pgfplots}
\pgfplotsset{compat=1.13}
 \geometry{
 a4paper,
 total={210mm,297mm},
 left=10mm,
 right=10mm,
 top=10mm,
 bottom=10mm,
 }
 % Write both of your names here. Fill exxxxxxx with your ceng mail address.
 \author{
  Öztürk, Kürşat\\
  \texttt{e2171874@ceng.metu.edu.tr}
  \and
  Burhan, Beste\\
  \texttt{e2171395@ceng.metu.edu.tr}
}
\title{CENG 384 - Signals and Systems for Computer Engineers \\
Spring 2018-2019 \\
Written Assignment 1}
\begin{document}
\maketitle



\noindent\rule{19cm}{1.2pt}

\begin{enumerate}

\item 
    \begin{enumerate}
    % Write your solutions in the following items.
    \item %write the solution of q1a
    \ \\
    $y(t)= \int_{}^{} (x(t)-4y(t))dt$\\
    $\dfrac{dy(t)}{dt} = x(t)-4y(t)$\\
    $\dot{y}(t)+ 4y(t) = x(t)$
    \item %write the solution of q1b
    \ \\
    $y(t) = y_h(t)+y_p(t)$\\
    Since initially at rest ;
    
    \ \ $y(0)=\dot{y}(0)=\ddot{y}(0)=.. = 0$\\
    Homogeneous solution;\\
    \null \ \ $y_h(t) = Ke^{\alpha t}$\\
    \null \ \ $(K\alpha+4K) e^{\alpha t}$\\\
    \null  \ \ $\alpha = -4$\\
    \null \ \ $y_h(t) = Ke^{-4t}$\\
    Particular solution;\\
    \null \ \ $x(t) = (e^{-t}+e^{-2t})u(t)$\\
    \null \ \ $ y_p(t) = a e^{-t}+be^{-2t}$ , \ \quad for $t>0$\\
    \null \ \ $ -ae^{-t}-2b e^{-2t}+4ae^{-t}+4b e^{-2t}= e^{-t}+e^{-2t}$\\
    \null \ \ $ 3a e^{-t}+ 2b e^{-2t}= e^{-t}+e^{-2t}$\\
    \null \ \ $a=1/3 \quad b=1/2$\\
    \null \ \ $ y_p(t) = \dfrac{1}{3}e^{-t}+\dfrac{1}{2}e^{-2t}$, \ \quad for $t>0$\\
    
    $y(t)= Ke^{-4t}+\dfrac{1}{3}e^{-t}+\dfrac{1}{2}e^{-2t}$, \ \quad for $t>0$\\
    $y(0)=0$\\
    $0=K+\dfrac{1}{3}+\dfrac{1}{2}$\\
    $K=-5/6$\\
    $y(t)=\Big[ \dfrac{-5}{6}e^{-4t}+\dfrac{1}{3}e^{-t}+\dfrac{1}{2}e^{-2t}\Big]u(t)$

\end{enumerate}


\item %write the solution of q2
\ \\
	\begin{enumerate}
		\item 
		\ \\ 
		$x[n] = \delta[n-1]-3\delta[n-2]+\delta[n-3]$\\
		$h[n] = \delta[n+1]+2\delta[n]-3\delta[n-1]$\\
		\ \\
		$y[n]=x[n]*h[n]=\sum_{k=-\infty}^{\infty}h[k]x[n-k]$\\
		$y[n]=h[-1]x[n+1]+h[0]x[n]+h[1]x[n-1]$\\
		\null \qquad $=x[n+1]+2x[n]+3x[n-1]$\\
		$y[n]=(\delta[n] - 3\delta[n-1]+\delta[n-2])+(2\delta[n-1]-6\delta[n-2]+2\delta[n-3])+(-3\delta[n-2]+9\delta[n-3]-3\delta[n-4])$\\
		\null \qquad $=\delta[n]-\delta[n-1]-8\delta[n-2]+11\delta[n-3]-3[n-4]$\\
		\ \\
		\begin{figure}[h!]
			\centering
			\begin{tikzpicture}[scale=1.1] 
			\begin{axis}[
			axis lines=middle,
			xlabel={$n$},
			ylabel={$\boldsymbol{y[n]}$},
			xtick={ -1,0,1,2,3,4,5},
			ytick={-8,-7,-6,...,-2,-1,-0,1,...,11},
			ymin=-8, ymax=11,
			xmin=-1, xmax=5,
			every axis x label/.style={at={(ticklabel* cs:1.05)}, anchor=west,},
			every axis y label/.style={at={(ticklabel* cs:1.05)}, anchor=south,},
			grid,	]
			\addplot [ycomb, black, thick, mark=*] table [x={n}, y={yn}] {q2a.dat};
			\end{axis}
			\end{tikzpicture}
			\caption{$y[n]=\delta[n]-\delta[n-1]-8\delta[n-2]+11\delta[n-3]-3[n-4]$.}
			\label{fig:q1}
		\end{figure}\\
	\null \\
	\null \\
	
		\item 
		\ \\
		$x(t)=u(t)+u(t-1)$\\
		$h(t)=(e^{-2t}cost )u(t)$\\
		$\dfrac{dx(t)}{dt}=\delta(t)+\delta(t-1)$\\
		$y(t)=\dfrac{dx(t)}{dt}*h(t)=\int_{0}^{\infty}e^{-2\tau}cos\tau \delta(t-\tau)d\tau + \int_{0}^{\infty}e^{-2\tau}cos\tau \delta(t-1-\tau)d\tau$\\
		\null \qquad \qquad \qquad \qquad \ = $e^{-2t}cost u(t) + e^{-2(t-1)}cos(t-1)u(t-1)$
	\end{enumerate}
\item  
\ \\
\begin{enumerate}
	\item %write the solution of q4a
	\ \\
	$x(t)=e^{-t}u(t)$\\
	$h(t)= e^{-3t}u(t)$\\
	
	$y(t)=x(t)*h(t)=\int_{0}^{t} e^{-\tau}e^{-3(t-\tau)}d\tau$\\
	\null \qquad \qquad \qquad \quad \ \ =$ e^{-3t}\int_{0}^{t}e^{2\tau}d\tau$\\
	\null \qquad \qquad \qquad \quad \ \ =$ e^{-3t}\Big(\dfrac{e^{2t}}{2}- \dfrac{1}{2}\Big) $\\
	$y(t)$=$\Big[\dfrac{e^{-t}}{2}-\dfrac{e^{-3t}}{2}\Big]u(t)$\\
	
	\item %write the solution of q4b
	\ \\
	$x(t)=u(t-1)-u(t-2)$\\
	$h(t)=e^tu(t)$\\
	
	$y(t)=x(t)*h(t)=\int_{-\infty}^{\infty}h(\tau)x(t-\tau)d\tau$\\
	\null \qquad \qquad \qquad \quad \ \ = $\int_{0}^{\infty}e^\tau(u(t-\tau-1)-u(t-\tau-2))d\tau$\\
	\null \qquad $t\le 1$,this convolution evalutates zero.\\
	For $1< t \le 2$\\
	\null \qquad \qquad $y(t)= \int_{0}^{t-1}e^\tau d\tau = e^{t-1}-1$\\
	For $t>2$\\
	\null \qquad \qquad $y(t) = \int_{t-2}^{t-1}e^\tau d\tau = e^{t-1}-e^{t-2}$\\
	
		\[   
		y(t) = 
		\begin{cases}
		\text{0,} & -\infty < t \le1\\
		e^{t-1}-1, & 1 < t \le 2 \\
		e^{t-1}-e^{t-2} &2 < t < \infty\\
		\end{cases}
		\]
\end{enumerate}
\item %write the solution of q5
\ \\
\begin{enumerate}
	\item %write the solution of q4c
	\ \\
	$y[n]-15y[n-1]+26y[n-2]=0$ \qquad $y[0]=10 , y[1]=42$\\
	Characteristic equation;\\
	\null \qquad $r^2-15r+26=0$\\
	\null \qquad $r_1=13$, $r_2 = 2$\\
	$y[n] = A(2)^n+B(13)^n$\\
	$y[0]=A+B = 10$\\
	$y[1]=A2+B13 = 42$\\
	$B=2,A=8$\\
	$y[n]=8.2^n+2.13^n$\\
	\item %write the solution of q4c
	\ \\
	$y[n]-3y[n-1]+y[n-2]=0$ \qquad $y[0]=1$, $y[1]=2$\\
	Characteristic equation;\\
	\null \qquad $r^2-3r+1=0$\\
	\null \qquad $r_1=\dfrac{3-\sqrt{5}}{2}$, $r_2=\dfrac{3+\sqrt{5}}{2}$\\
	$y[n]= A \Big(\dfrac{3-\sqrt{5}}{2}\Big)^n + B\Big(\dfrac{3+\sqrt{5}}{2}\Big)^n$\\
	$y[0]= A+B = 1$\\
	$y[1]= A\Big(\dfrac{3-\sqrt{5}}{2}\Big)+B\Big(\dfrac{3+\sqrt{5}}{2}\Big)=2$\\
	$B=\dfrac{5+\sqrt{5}}{10}$, $A==\dfrac{5-\sqrt{5}}{10}$\\
	$y[n]= \dfrac{5-\sqrt{5}}{10} \Big(\dfrac{3-\sqrt{5}}{2}\Big)^n + \dfrac{5+\sqrt{5}}{10} \Big(\dfrac{3+\sqrt{5}}{2}\Big)^n $
\end{enumerate}
\item 
\ \\
    \begin{enumerate}
    \item %write the solution of q4a
    \ \\
    $\ddot{y}(t)+6\dot{y}(t)+8y(t)=2x(t)$\\
    $x(t)=\delta(t)$\\
    $\ddot{h}(t)+6\dot{h}(t)+8h(t)=2\delta(t)$\\
    $h(t)=0 $ for $t<0$ \qquad \ \ $h(0^-)=0$, $\dot{h}(0^-)=0$\\
    For $t=0$\\
    \null \qquad $\int_{0^-}^{0^+}\ddot{h}(t)dt + 6 \int_{0^-}^{0^+}\dot{h}(t)dt + 8 \int_{0^-}^{0^+}h(t)dt = \null \qquad 2\int_{0^-}^{0^+}\delta(t)dt$\\
    \null \qquad $\dot{h}(0^+)-\dot{h}(0^-) + 6h(0^+)-6h(0^-)+0=2$\\
    \null \qquad $\dot{h}(0^+) - 6h(0^+) = 2 $\\
    \null \qquad $\dot{h}(0^+)=2$\\
   \null \qquad  $h(0^+) =0$ since the position $y(t)$ is not changed at $t=0$ so $y(0^+)=y(0^-)$\\
   For $t>0$ it must be solve;\\
   \null \qquad $ \ddot{h}+6 \dot{h}+8h=0$, $\dot{0^+}=2$, $h(0^+)=0$\\
   \null \qquad Characteristic equation;\\
   \null \qquad \qquad $r^2+6r+8=0$ \qquad $r_1=-4$, $r_2=-2$\\
   \null \qquad $h(t)=K_1e^{-4t}+K_2e^{-2t}$ \qquad for $ t> 0$\\
   \null \qquad\ \ \  0 = $h(0^+) = K_1 + K_2$\\
    \null \qquad\ \ \  2 = $\dot{h}(0^+)=-4K_1-2K_2$\\
     \null \qquad $K_1=-1$, $K_2=1$\\
     $h(t)=\Big[-e^{-4t}+e^{-2t}\Big] u(t)$
    
    \item %write the solution of q4b
    \ \\
    $h(t)=\Big[-e^{-4t}+e^{-2t}\Big] u(t)$
    	\begin{enumerate}
    		\item %write the solution of q4c
    		\ \\
    		Causal because $h(t)=0$ for $t<0$\\
    		\item %write the solution of q4c
    		\ \\
    		It has memory because when $\exists t \ne 0$ $ h(t) \ne 0$. For example $h(1)=-e^{-4}+e^{-2} \ne 0$
    		\item %write the solution of q4c
    		\ \\
    		Stable because $\int_{-\infty}^{\infty}|h(t)|dt=3/4 < \infty$
    		\item %write the solution of q4c
    		\ \\
    		It is invertible
		\end{enumerate}
    \end{enumerate}



\end{enumerate}
\end{document}

